work on building

src/burrow/building.v
@@ -14,18 +14,193 @@ Require Import Burrow.rollup.
 Require Import Burrow.indexing.
 Require Import Burrow.locations.
 
-Definition build {RI} `{!EqDecision RI} `{!Countable RI} {M} `{!EqDecision M, !TPCM M}
-    (loc: Loc RI) (cell: Cell M) : Branch M. Admitted.
-    
-Lemma build_spec {RI} `{!EqDecision RI} `{!Countable RI} {M} `{!EqDecision M, !TPCM M}
-    (loc: Loc RI) (cell: Cell M)
-  : (∀ pl , pl ∈ pls_of_loc loc -> cell_of_pl (build loc cell) pl ≡ cell). Admitted.
+Section BuildOne.
+  Context {M} `{!EqDecision M, !TPCM M}.
+
+  Fixpoint unwalk (j: nat) (b: Branch M) :=
+    match j with
+    | 0 => b
+    | S j => unwalk j (BranchCons triv_node b)
+    end.
   
-Lemma build_rest_triv
-        {M} `{!EqDecision M, !TPCM M}
-        {RI} `{!EqDecision RI, !Countable RI}
-    (loc: Loc RI) (cell: Cell M)
-  : (∀ pl , ¬(pl ∈ pls_of_loc loc) -> cell_of_pl (build loc cell) pl ≡ triv_cell). Admitted.
+  Definition unhop (j: nat) (b: Branch M) :=
+    unwalk j (BranchCons (CellNode triv_cell b) BranchNil).
+  
+  Fixpoint unhops (js: list nat) (b: Branch M) :=
+    match js with
+    | [] => b
+    | (j :: ks) => unhop j (unhops ks b)
+    end.
+  
+  Definition build_of_branch (branch: Branch M) (pl: PathLoc) : Branch M :=
+    match pl with
+    | (p, i) => unhops p (unwalk i branch)
+    end.
+  
+  Definition build_of_node (node: Node M) (pl: PathLoc) : Branch M :=
+    build_of_branch (BranchCons node BranchNil) pl.
+    
+  Definition build_of_cell (cell: Cell M) (pl: PathLoc) : Branch M :=
+    build_of_node (CellNode cell BranchNil) pl.
+    
+  Lemma walk_unwalk (branch: Branch M) j
+    : walk j (unwalk j branch) = branch.
+  Proof.
+    generalize branch. clear branch.
+    induction j; trivial.
+    cbn [walk]. cbn [unwalk]. intro. rewrite IHj. unfold branch_of_branch. trivial. Qed.
+    
+  Lemma hop_unhop (branch: Branch M) j
+    : hop j (unhop j branch) = branch.
+  Proof.
+    unfold hop, unhop. rewrite walk_unwalk. unfold node_of_branch, branch_of_node.
+    trivial. Qed.
+    
+  Lemma hops_unhops (branch: Branch M) js
+    : hops js (unhops js branch) = branch.
+  Proof.
+    generalize branch. clear branch.
+    induction js; trivial.
+    cbn [hops]. cbn [unhops]. intro. rewrite hop_unhop. rewrite IHjs. trivial. Qed.
+    
+  Lemma branch_of_pl_build_of_branch (branch: Branch M) (pl: PathLoc)
+    : branch_of_pl (build_of_branch branch pl) pl = branch.
+  Proof.
+    unfold branch_of_pl, build_of_branch. destruct pl. rewrite hops_unhops.
+      rewrite walk_unwalk. trivial. Qed.
+    
+  Lemma node_of_pl_build_of_node (node: Node M) (pl: PathLoc)
+    : node_of_pl (build_of_node node pl) pl = node.
+  Proof.
+    unfold node_of_pl, build_of_node.
+    rewrite branch_of_pl_build_of_branch. unfold node_of_branch. trivial. Qed.
+    
+  Lemma cell_of_pl_build_of_cell (cell: Cell M) (pl: PathLoc)
+    : cell_of_pl (build_of_cell cell pl) pl = cell.
+  Proof.
+    unfold cell_of_pl. unfold build_of_cell. rewrite node_of_pl_build_of_node.
+    unfold cell_of_node. trivial. Qed.
+    
+  Lemma unwalk_add p q b
+  : unwalk (p + q) b = unwalk q (unwalk p b).
+  Proof. generalize b. clear b. induction p.
+    - trivial.
+    - intro. replace (S p + q) with (S (p + q)) by lia.
+      cbn [unwalk]. rewrite IHp. trivial.
+  Qed.
+  
+  Lemma node_of_branch_unwalk_nonzero j b
+    (nz: j ≠ 0) : node_of_branch (unwalk j b) = triv_node.
+  Proof.
+    generalize b. clear b. induction j.
+    - contradiction.
+    - cbn [unwalk]. destruct j.
+      + unfold unwalk. unfold node_of_branch. trivial.
+      + intro. apply IHj. lia.
+  Qed.
+  
+  Lemma walk_eq_BranchNil_nonzero j n
+    (nz: j ≠ 0) : (walk j (BranchCons n BranchNil)) = BranchNil.
+  Proof.
+    induction j.
+    - contradiction.
+    - cbn [walk]. destruct j.
+      + trivial.
+      + rewrite IHj; trivial. lia.
+  Qed.
+
+  Lemma node_of_branch_walk_nonzero j n
+    (nz: j ≠ 0) : node_of_branch (walk j (BranchCons n BranchNil)) = triv_node.
+  Proof.
+    rewrite walk_eq_BranchNil_nonzero; trivial.
+  Qed.
+
+  Lemma node_of_branch_walk_unwalk_i_ne (n: Node M) (i i': nat)
+    (ne : i ≠ i')
+    : node_of_branch (walk i (unwalk i' (BranchCons n BranchNil))) = triv_node.
+  Proof.
+    have h : Decision (i < i') by solve_decision. destruct h.
+    - replace i' with ((i' - i) + i) by lia.
+      rewrite unwalk_add. rewrite walk_unwalk.
+      apply node_of_branch_unwalk_nonzero. lia.
+    - replace i with (i' + (i - i')) by lia.
+      rewrite walk_add. rewrite walk_unwalk.
+      apply node_of_branch_walk_nonzero. lia.
+  Qed.
+    
+  Lemma node_of_pl_build_of_cell_i_ne (node: Node M) (p : list nat) (i i' : nat)
+    (ne: i ≠ i')
+    : node_of_pl (build_of_node node (p, i')) (p, i) = triv_node.
+  Proof.
+    unfold node_of_pl, build_of_node. 
+    unfold branch_of_pl, build_of_branch.
+    rewrite hops_unhops. apply node_of_branch_walk_unwalk_i_ne. trivial.
+  Qed.
+    
+  Lemma cell_of_pl_build_of_cell_i_ne (cell: Cell M) (p : list nat) (i i' : nat)
+    (ne: i ≠ i')
+    : cell_of_pl (build_of_cell cell (p, i')) (p, i) = triv_cell.
+  Proof.
+    unfold cell_of_pl, build_of_cell. rewrite node_of_pl_build_of_cell_i_ne; trivial.
+  Qed.
+    
+  Lemma cell_of_pl_build_of_cell_p_ne (cell: Cell M) (p p' : list nat) (i i' : nat)
+    (ne: p ≠ p')
+    : cell_of_pl (build_of_cell cell (p, i')) (p', i) = triv_cell. Admitted.
+    
+  Lemma cell_of_pl_build_of_cell_ne (cell: Cell M) (pl pl': PathLoc)
+    (ne: pl ≠ pl')
+    : cell_of_pl (build_of_cell cell pl') pl = triv_cell.
+  Proof.
+    generalize ne. generalize pl'. clear ne. clear pl'.
+    destruct pl. rename l into p. rename n into i.
+    destruct pl'. rename l into p'. rename n into i'.
+    intro.
+    have h : Decision (p = p') by solve_decision. destruct h.
+    - subst p'. assert (i ≠ i') by intuition.
+      apply cell_of_pl_build_of_cell_i_ne; trivial.
+    - apply cell_of_pl_build_of_cell_p_ne; trivial. crush.
+  Qed.
+    
+End BuildOne.
+
+Section Build.
+  Context {RI} `{!EqDecision RI} `{!Countable RI} {M} `{!EqDecision M, !TPCM M}.
+
+  Definition buildfn cell : PathLoc -> Branch M -> Branch M :=
+      (λ pl b , b ⋅ build_of_cell cell pl).
+
+  Definition build (loc: Loc RI) (cell: Cell M) : Branch M :=
+    set_fold (buildfn cell) BranchNil (pls_of_loc loc).
+    
+  Lemma cell_of_pl_set_fold_not_in (cell: Cell M) (s: gset PathLoc) (pl: PathLoc)
+    (is_in: pl ∉ s)
+    : cell_of_pl (set_fold (buildfn cell) BranchNil s) pl ≡ triv_cell.
+  Proof. apply set_easy_induct_strong.
+    - unfold cell_of_pl. unfold node_of_pl. setoid_rewrite branch_of_pl_BranchNil.
+        unfold node_of_branch. unfold cell_of_node, triv_node. trivial.
+    - intros. unfold buildfn. setoid_rewrite <- cell_of_pl_op.
+      assert (pl ≠ a) by crush.
+      rewrite cell_of_pl_build_of_cell_ne; trivial.
+      setoid_rewrite H0. apply op_trivial_cell. unfold cell_trivial, triv_cell. intuition.
+  Qed.
+
+  Lemma cell_of_pl_set_fold_in (cell: Cell M) (s: gset PathLoc) (pl: PathLoc)
+    (is_in: pl ∈ s)
+    : cell_of_pl (set_fold (buildfn cell) BranchNil s) pl ≡ cell. Admitted.
+    
+  Lemma build_spec
+      (loc: Loc RI) (cell: Cell M)
+    : (∀ pl , pl ∈ pls_of_loc loc -> cell_of_pl (build loc cell) pl ≡ cell).
+  Proof.
+    intros. unfold build. apply cell_of_pl_set_fold_in. trivial. Qed.
+  
+  Lemma build_rest_triv
+      (loc: Loc RI) (cell: Cell M)
+    : (∀ pl , ¬(pl ∈ pls_of_loc loc) -> cell_of_pl (build loc cell) pl ≡ triv_cell).
+  Proof.
+    intros. unfold build. apply cell_of_pl_set_fold_not_in. trivial. Qed.
+End Build.
 
 Global Instance build_proper
     {M} `{!EqDecision M, !TPCM M}
